lectures/PulseIntro.fst
@@ -4,6 +4,22 @@ open Pulse
 
 let fstar_five : int = 5
 
+(*
+
+Separation Logic Primer
+-----------------------
+
+{ P } c { \v. Q }
+
+where `P` and `Q` are separation logic predicates `slprop`s. `slprop` stands for
+separation logic predicates.
+
+type slprop = state -> prop
+
+where `state` is the state of the heap.
+
+*)
+
 fn five ()
   requires emp
   returns n:int
@@ -13,5 +29,108 @@ fn five ()
 }
 
 let pulse_five_in_fstar = five ()
-
 let pulse_five : int = 5
+
+(*
+
+The above is a convenient way to write
+
+```
+{ emp } five () { n:int. pure (n == 5) }.
+```
+
+*)
+
+(*
+
+Some simple slprops:
+--------------------
+* `emp`, the trivial proposition (equivalent to `fun s -> True`).
+* `pure p`, heap-independent predicate `fun s -> p`.
+   + `emp` is equivalent to `pure True`.
+
+Ownership and permission
+------------------------
+* Key idea is the concept of ownership.
+  + A computation can only access those resources that it is explicitly granted
+    access to in its precondition or those that it creates itself.
+  + `five` cannot access any resources, because its precondition is `emp`.
+    - This is different from ST effect in F*. See `incr` in
+      `PureIntroSupport.fst`.
+*)
+
+(* UNCOMMENT AND EXPECT FAILURE *)
+(*
+fn five' (x : ref int)
+  requires emp
+  returns n:int
+  ensures pure (n == 5)
+{
+  let v = !x;
+  x := v + 1;
+  fstar_five
+}
+*)
+
+fn incr (x:ref int)
+requires pts_to x 'i
+ensures pts_to x ('i + 1)
+{
+    let v = !x;
+    x := v + 1;
+}
+
+(*
+
+Separation Logic Rules
+----------------------
+
+## Connectives in Separation Logic
+
+Connectives of separation logic in terms of the sets of partial
+heaps that they accept.
+
+(1) emp = {●}
+(2) pts_to x v = {●[x -> v]}
+(3) pure P = {h | P /\ h = ●}
+(3) exists x. P = {h | exists x. h ∈ P(x)}
+(4) P ** Q = {h1 ⨄ h2 | h1 ∈ P /\ h2 ∈ Q}
+(5) p @==> q = {h | h ∈ p ==> h ∈ q}
+
+## Properties
+
+* Commutative : P ** Q @==> Q ** P
+* Associative : P ** (Q ** R) @==> (P ** Q) ** R
+* Idempotent  : P ** emp @==> P
+* Frame rule  :
+
+       {P} c {Q}
+  -------------------
+  {P ** R} c {Q ** R}
+
+  + Captures the essence of local modular reasoning
+  + If a program is correct with permission `P` then it is correct in a larger
+    context with additional permissions `R` which it doesn't touch.
+
+*)
+
+(* Thanks to the frame rule, the following need not mention anything about `y`.
+   This is not true with ST effect in F*. See `incr3` in
+   `PulseIntroSupport.fst` *)
+
+fn incr_frame (x y:ref int)
+requires pts_to x 'i ** pts_to y 'j
+ensures pts_to x ('i + 1) ** pts_to y 'j
+{
+   incr x;
+}
+
+(* In fact, Pulse lets us use the frame rule with any `f:slprop`, and we get,
+   for free, that `incr x` does not disturb `f`. *)
+
+fn incr_frame_any (x:ref int) (f:slprop)
+requires pts_to x 'i ** f
+ensures pts_to x ('i + 1) ** f
+{
+   incr x;
+}
