lectures/PulseIntroSupport.fst
@@ -1,0 +1,22 @@
+module PulseIntroSupport
+
+open FStar.All
+open FStar.Ref
+
+val incr : r:ref int -> FStar.All.St unit
+let incr r =
+  (r := (!r + 1))
+
+val incr2 : r:ref int -> ST unit (requires (fun h0 -> True))
+  (ensures (fun h0 _ h2 ->
+    modifies !{r} h0 h2 /\
+    sel h2 r == sel h0 r + 1))
+let incr2 r = r := !r + 1
+
+val incr3 : x:ref int -> y:ref int -> ST unit
+  (requires (fun h0 -> addr_of x <> addr_of y)) (* Non-aliasing is necessary *)
+  (ensures (fun h0 _ h2 ->
+    modifies !{x} h0 h2 /\
+    sel h2 x == sel h0 x + 1 /\
+    sel h2 y == sel h0 y))
+let incr3 x y = x := !x + 1
